base_logic/lib/sts.v
@@ -22,7 +22,7 @@ Section definitions.
   Definition sts_own (s : sts.state sts) (T : sts.tokens sts) : iProp Σ :=
     own γ (sts_frag_up s T).
   Definition sts_inv (φ : sts.state sts → iProp Σ) : iProp Σ :=
-    (∃ s, own γ (sts_auth s ∅) ★ φ s)%I.
+    (∃ s, own γ (sts_auth s ∅) ∗ φ s)%I.
   Definition sts_ctx (N : namespace) (φ: sts.state sts → iProp Σ) : iProp Σ :=
     inv N (sts_inv φ).
 
@@ -68,21 +68,21 @@ Section sts.
      sts_frag_included. *)
   Lemma sts_ownS_weaken γ S1 S2 T1 T2 :
     T2 ⊆ T1 → S1 ⊆ S2 → sts.closed S2 T2 →
-    sts_ownS γ S1 T1 ==★ sts_ownS γ S2 T2.
+    sts_ownS γ S1 T1 ==∗ sts_ownS γ S2 T2.
   Proof. intros ???. by apply own_update, sts_update_frag. Qed.
 
   Lemma sts_own_weaken γ s S T1 T2 :
     T2 ⊆ T1 → s ∈ S → sts.closed S T2 →
-    sts_own γ s T1 ==★ sts_ownS γ S T2.
+    sts_own γ s T1 ==∗ sts_ownS γ S T2.
   Proof. intros ???. by apply own_update, sts_update_frag_up. Qed.
 
   Lemma sts_ownS_op γ S1 S2 T1 T2 :
     T1 ⊥ T2 → sts.closed S1 T1 → sts.closed S2 T2 →
-    sts_ownS γ (S1 ∩ S2) (T1 ∪ T2) ⊣⊢ (sts_ownS γ S1 T1 ★ sts_ownS γ S2 T2).
+    sts_ownS γ (S1 ∩ S2) (T1 ∪ T2) ⊣⊢ (sts_ownS γ S1 T1 ∗ sts_ownS γ S2 T2).
   Proof. intros. by rewrite /sts_ownS -own_op sts_op_frag. Qed.
 
   Lemma sts_alloc E N s :
-    ▷ φ s ={E}=★ ∃ γ, sts_ctx γ N φ ∧ sts_own γ s (⊤ ∖ sts.tok s).
+    ▷ φ s ={E}=∗ ∃ γ, sts_ctx γ N φ ∧ sts_own γ s (⊤ ∖ sts.tok s).
   Proof.
     iIntros "Hφ". rewrite /sts_ctx /sts_own.
     iMod (own_alloc (sts_auth s (⊤ ∖ sts.tok s))) as (γ) "Hγ".
@@ -93,9 +93,9 @@ Section sts.
   Qed.
 
   Lemma sts_accS E γ S T :
-    ▷ sts_inv γ φ ★ sts_ownS γ S T ={E}=★ ∃ s,
-      ■ (s ∈ S) ★ ▷ φ s ★ ∀ s' T',
-      ■ sts.steps (s, T) (s', T') ★ ▷ φ s' ={E}=★ ▷ sts_inv γ φ ★ sts_own γ s' T'.
+    ▷ sts_inv γ φ ∗ sts_ownS γ S T ={E}=∗ ∃ s,
+      ■ (s ∈ S) ∗ ▷ φ s ∗ ∀ s' T',
+      ■ sts.steps (s, T) (s', T') ∗ ▷ φ s' ={E}=∗ ▷ sts_inv γ φ ∗ sts_own γ s' T'.
   Proof.
     iIntros "[Hinv Hγf]". rewrite /sts_ownS /sts_inv /sts_own.
     iDestruct "Hinv" as (s) "[>Hγ Hφ]".
@@ -111,16 +111,16 @@ Section sts.
   Qed.
 
   Lemma sts_acc E γ s0 T :
-    ▷ sts_inv γ φ ★ sts_own γ s0 T ={E}=★ ∃ s,
-      ■ sts.frame_steps T s0 s ★ ▷ φ s ★ ∀ s' T',
-      ■ sts.steps (s, T) (s', T') ★ ▷ φ s' ={E}=★ ▷ sts_inv γ φ ★ sts_own γ s' T'.
+    ▷ sts_inv γ φ ∗ sts_own γ s0 T ={E}=∗ ∃ s,
+      ■ sts.frame_steps T s0 s ∗ ▷ φ s ∗ ∀ s' T',
+      ■ sts.steps (s, T) (s', T') ∗ ▷ φ s' ={E}=∗ ▷ sts_inv γ φ ∗ sts_own γ s' T'.
   Proof. by apply sts_accS. Qed.
 
   Lemma sts_openS E N γ S T :
     nclose N ⊆ E →
-    sts_ctx γ N φ ★ sts_ownS γ S T ={E,E∖N}=★ ∃ s,
-      ■ (s ∈ S) ★ ▷ φ s ★ ∀ s' T',
-      ■ sts.steps (s, T) (s', T') ★ ▷ φ s' ={E∖N,E}=★ sts_own γ s' T'.
+    sts_ctx γ N φ ∗ sts_ownS γ S T ={E,E∖N}=∗ ∃ s,
+      ■ (s ∈ S) ∗ ▷ φ s ∗ ∀ s' T',
+      ■ sts.steps (s, T) (s', T') ∗ ▷ φ s' ={E∖N,E}=∗ sts_own γ s' T'.
   Proof.
     iIntros (?) "[#? Hγf]". rewrite /sts_ctx. iInv N as "Hinv" "Hclose".
     (* The following is essentially a very trivial composition of the accessors
@@ -136,8 +136,8 @@ Section sts.
 
   Lemma sts_open E N γ s0 T :
     nclose N ⊆ E →
-    sts_ctx γ N φ ★ sts_own γ s0 T ={E,E∖N}=★ ∃ s,
-      ■ (sts.frame_steps T s0 s) ★ ▷ φ s ★ ∀ s' T',
-      ■ (sts.steps (s, T) (s', T')) ★ ▷ φ s' ={E∖N,E}=★ sts_own γ s' T'.
+    sts_ctx γ N φ ∗ sts_own γ s0 T ={E,E∖N}=∗ ∃ s,
+      ■ (sts.frame_steps T s0 s) ∗ ▷ φ s ∗ ∀ s' T',
+      ■ (sts.steps (s, T) (s', T')) ∗ ▷ φ s' ={E∖N,E}=∗ sts_own γ s' T'.
   Proof. by apply sts_openS. Qed.
 End sts.
