base_logic/lib/wsat.v
@@ -36,8 +36,8 @@ Instance: Params (@ownD) 3.
 
 Definition wsat `{invG Σ} : iProp Σ :=
   (∃ I : gmap positive (iProp Σ),
-    own invariant_name (● (invariant_unfold <$> I : gmap _ _)) ★
-    [★ map] i ↦ Q ∈ I, ▷ Q ★ ownD {[i]} ∨ ownE {[i]})%I.
+    own invariant_name (● (invariant_unfold <$> I : gmap _ _)) ∗
+    [∗ map] i ↦ Q ∈ I, ▷ Q ∗ ownD {[i]} ∨ ownE {[i]})%I.
 
 Section wsat.
 Context `{invG Σ}.
@@ -52,40 +52,40 @@ Qed.
 Global Instance ownI_persistent i P : PersistentP (ownI i P).
 Proof. rewrite /ownI. apply _. Qed.
 
-Lemma ownE_empty : True ==★ ownE ∅.
+Lemma ownE_empty : True ==∗ ownE ∅.
 Proof. by rewrite (own_empty (A:=coPset_disjUR) enabled_name). Qed.
-Lemma ownE_op E1 E2 : E1 ⊥ E2 → ownE (E1 ∪ E2) ⊣⊢ ownE E1 ★ ownE E2.
+Lemma ownE_op E1 E2 : E1 ⊥ E2 → ownE (E1 ∪ E2) ⊣⊢ ownE E1 ∗ ownE E2.
 Proof. intros. by rewrite /ownE -own_op coPset_disj_union. Qed.
-Lemma ownE_disjoint E1 E2 : ownE E1 ★ ownE E2 ⊢ E1 ⊥ E2.
+Lemma ownE_disjoint E1 E2 : ownE E1 ∗ ownE E2 ⊢ E1 ⊥ E2.
 Proof. rewrite /ownE own_valid_2. by iIntros (?%coPset_disj_valid_op). Qed.
-Lemma ownE_op' E1 E2 : E1 ⊥ E2 ∧ ownE (E1 ∪ E2) ⊣⊢ ownE E1 ★ ownE E2.
+Lemma ownE_op' E1 E2 : E1 ⊥ E2 ∧ ownE (E1 ∪ E2) ⊣⊢ ownE E1 ∗ ownE E2.
 Proof.
   iSplit; [iIntros "[% ?]"; by iApply ownE_op|].
   iIntros "HE". iDestruct (ownE_disjoint with "HE") as %?.
   iSplit; first done. iApply ownE_op; by try iFrame.
 Qed.
-Lemma ownE_singleton_twice i : ownE {[i]} ★ ownE {[i]} ⊢ False.
+Lemma ownE_singleton_twice i : ownE {[i]} ∗ ownE {[i]} ⊢ False.
 Proof. rewrite ownE_disjoint. iIntros (?); set_solver. Qed.
 
-Lemma ownD_empty : True ==★ ownD ∅.
+Lemma ownD_empty : True ==∗ ownD ∅.
 Proof. by rewrite (own_empty (A:=gset_disjUR _) disabled_name). Qed.
-Lemma ownD_op E1 E2 : E1 ⊥ E2 → ownD (E1 ∪ E2) ⊣⊢ ownD E1 ★ ownD E2.
+Lemma ownD_op E1 E2 : E1 ⊥ E2 → ownD (E1 ∪ E2) ⊣⊢ ownD E1 ∗ ownD E2.
 Proof. intros. by rewrite /ownD -own_op gset_disj_union. Qed.
-Lemma ownD_disjoint E1 E2 : ownD E1 ★ ownD E2 ⊢ E1 ⊥ E2.
+Lemma ownD_disjoint E1 E2 : ownD E1 ∗ ownD E2 ⊢ E1 ⊥ E2.
 Proof. rewrite /ownD own_valid_2. by iIntros (?%gset_disj_valid_op). Qed.
-Lemma ownD_op' E1 E2 : E1 ⊥ E2 ∧ ownD (E1 ∪ E2) ⊣⊢ ownD E1 ★ ownD E2.
+Lemma ownD_op' E1 E2 : E1 ⊥ E2 ∧ ownD (E1 ∪ E2) ⊣⊢ ownD E1 ∗ ownD E2.
 Proof.
   iSplit; [iIntros "[% ?]"; by iApply ownD_op|].
   iIntros "HE". iDestruct (ownD_disjoint with "HE") as %?.
   iSplit; first done. iApply ownD_op; by try iFrame.
 Qed.
-Lemma ownD_singleton_twice i : ownD {[i]} ★ ownD {[i]} ⊢ False.
+Lemma ownD_singleton_twice i : ownD {[i]} ∗ ownD {[i]} ⊢ False.
 Proof. rewrite ownD_disjoint. iIntros (?); set_solver. Qed.
 
 Lemma invariant_lookup (I : gmap positive (iProp Σ)) i P :
-  own invariant_name (● (invariant_unfold <$> I : gmap _ _)) ★
+  own invariant_name (● (invariant_unfold <$> I : gmap _ _)) ∗
   own invariant_name (◯ {[i := invariant_unfold P]}) ⊢
-  ∃ Q, I !! i = Some Q ★ ▷ (Q ≡ P).
+  ∃ Q, I !! i = Some Q ∗ ▷ (Q ≡ P).
 Proof.
   rewrite own_valid_2 auth_validI /=. iIntros "[#HI #HvI]".
   iDestruct "HI" as (I') "HI". rewrite gmap_equivI gmap_validI.
@@ -101,7 +101,7 @@ Proof.
   by rewrite agree_equivI uPred.later_equivI iProp_unfold_equivI.
 Qed.
 
-Lemma ownI_open i P : wsat ★ ownI i P ★ ownE {[i]} ⊢ wsat ★ ▷ P ★ ownD {[i]}.
+Lemma ownI_open i P : wsat ∗ ownI i P ∗ ownE {[i]} ⊢ wsat ∗ ▷ P ∗ ownD {[i]}.
 Proof.
   rewrite /ownI. iIntros "(Hw & Hi & HiE)". iDestruct "Hw" as (I) "[? HI]".
   iDestruct (invariant_lookup I i P with "[$Hw $Hi]") as (Q) "[% #HPQ]".
@@ -111,7 +111,7 @@ Proof.
     iFrame "HI"; eauto.
   - iDestruct (ownE_singleton_twice with "[$HiE $HiE']") as %[].
 Qed.
-Lemma ownI_close i P : wsat ★ ownI i P ★ ▷ P ★ ownD {[i]} ⊢ wsat ★ ownE {[i]}.
+Lemma ownI_close i P : wsat ∗ ownI i P ∗ ▷ P ∗ ownD {[i]} ⊢ wsat ∗ ownE {[i]}.
 Proof.
   rewrite /ownI. iIntros "(Hw & Hi & HP & HiD)". iDestruct "Hw" as (I) "[? HI]".
   iDestruct (invariant_lookup with "[$Hw $Hi]") as (Q) "[% #HPQ]".
@@ -123,7 +123,7 @@ Qed.
 
 Lemma ownI_alloc φ P :
   (∀ E : gset positive, ∃ i, i ∉ E ∧ φ i) →
-  wsat ★ ▷ P ==★ ∃ i, ■ (φ i) ★ wsat ★ ownI i P.
+  wsat ∗ ▷ P ==∗ ∃ i, ■ (φ i) ∗ wsat ∗ ownI i P.
 Proof.
   iIntros (Hfresh) "[Hw HP]". iDestruct "Hw" as (I) "[? HI]".
   iMod (own_empty (A:=gset_disjUR positive) disabled_name) as "HE".
