proofmode/class_instances.v
@@ -69,20 +69,20 @@ Global Instance into_later_or P1 P2 Q1 Q2 :
   IntoLater P1 Q1 → IntoLater P2 Q2 → IntoLater (P1 ∨ P2) (Q1 ∨ Q2).
 Proof. intros ??; red. by rewrite later_or; apply or_mono. Qed.
 Global Instance into_later_sep P1 P2 Q1 Q2 :
-  IntoLater P1 Q1 → IntoLater P2 Q2 → IntoLater (P1 ★ P2) (Q1 ★ Q2).
+  IntoLater P1 Q1 → IntoLater P2 Q2 → IntoLater (P1 ∗ P2) (Q1 ∗ Q2).
 Proof. intros ??; red. by rewrite later_sep; apply sep_mono. Qed.
 
 Global Instance into_later_big_sepM `{Countable K} {A}
     (Φ Ψ : K → A → uPred M) (m : gmap K A) :
   (∀ x k, IntoLater (Φ k x) (Ψ k x)) →
-  IntoLater ([★ map] k ↦ x ∈ m, Φ k x) ([★ map] k ↦ x ∈ m, Ψ k x).
+  IntoLater ([∗ map] k ↦ x ∈ m, Φ k x) ([∗ map] k ↦ x ∈ m, Ψ k x).
 Proof.
   rewrite /IntoLater=> ?. rewrite big_sepM_later; by apply big_sepM_mono.
 Qed.
 Global Instance into_later_big_sepS `{Countable A}
     (Φ Ψ : A → uPred M) (X : gset A) :
   (∀ x, IntoLater (Φ x) (Ψ x)) →
-  IntoLater ([★ set] x ∈ X, Φ x) ([★ set] x ∈ X, Ψ x).
+  IntoLater ([∗ set] x ∈ X, Φ x) ([∗ set] x ∈ X, Ψ x).
 Proof.
   rewrite /IntoLater=> ?. rewrite big_sepS_later; by apply big_sepS_mono.
 Qed.
@@ -97,12 +97,12 @@ Global Instance from_later_or P1 P2 Q1 Q2 :
   FromLater P1 Q1 → FromLater P2 Q2 → FromLater (P1 ∨ P2) (Q1 ∨ Q2).
 Proof. intros ??; red. by rewrite later_or; apply or_mono. Qed.
 Global Instance from_later_sep P1 P2 Q1 Q2 :
-  FromLater P1 Q1 → FromLater P2 Q2 → FromLater (P1 ★ P2) (Q1 ★ Q2).
+  FromLater P1 Q1 → FromLater P2 Q2 → FromLater (P1 ∗ P2) (Q1 ∗ Q2).
 Proof. intros ??; red. by rewrite later_sep; apply sep_mono. Qed.
 
 (* IntoWand *)
 Global Instance into_wand_wand P Q Q' :
-  FromAssumption false Q Q' → IntoWand (P -★ Q) P Q'.
+  FromAssumption false Q Q' → IntoWand (P -∗ Q) P Q'.
 Proof. by rewrite /FromAssumption /IntoWand /= => ->. Qed.
 Global Instance into_wand_impl P Q Q' :
   FromAssumption false Q Q' → IntoWand (P → Q) P Q'.
@@ -121,10 +121,10 @@ Proof. rewrite /IntoWand=>->. apply wand_intro_l. by rewrite bupd_wand_r. Qed.
 Global Instance from_and_and P1 P2 : FromAnd (P1 ∧ P2) P1 P2.
 Proof. done. Qed.
 Global Instance from_and_sep_persistent_l P1 P2 :
-  PersistentP P1 → FromAnd (P1 ★ P2) P1 P2 | 9.
+  PersistentP P1 → FromAnd (P1 ∗ P2) P1 P2 | 9.
 Proof. intros. by rewrite /FromAnd always_and_sep_l. Qed.
 Global Instance from_and_sep_persistent_r P1 P2 :
-  PersistentP P2 → FromAnd (P1 ★ P2) P1 P2 | 10.
+  PersistentP P2 → FromAnd (P1 ∗ P2) P1 P2 | 10.
 Proof. intros. by rewrite /FromAnd always_and_sep_r. Qed.
 Global Instance from_and_always P Q1 Q2 :
   FromAnd P Q1 Q2 → FromAnd (□ P) (□ Q1) (□ Q2).
@@ -134,7 +134,7 @@ Global Instance from_and_later P Q1 Q2 :
 Proof. rewrite /FromAnd=> <-. by rewrite later_and. Qed.
 
 (* FromSep *)
-Global Instance from_sep_sep P1 P2 : FromSep (P1 ★ P2) P1 P2 | 100.
+Global Instance from_sep_sep P1 P2 : FromSep (P1 ∗ P2) P1 P2 | 100.
 Proof. done. Qed.
 Global Instance from_sep_ownM (a b1 b2 : M) :
   FromOp a b1 b2 →
@@ -153,14 +153,14 @@ Proof. rewrite /FromSep=><-. apply bupd_sep. Qed.
 Global Instance from_sep_big_sepM
     `{Countable K} {A} (Φ Ψ1 Ψ2 : K → A → uPred M) m :
   (∀ k x, FromSep (Φ k x) (Ψ1 k x) (Ψ2 k x)) →
-  FromSep ([★ map] k ↦ x ∈ m, Φ k x)
-    ([★ map] k ↦ x ∈ m, Ψ1 k x) ([★ map] k ↦ x ∈ m, Ψ2 k x).
+  FromSep ([∗ map] k ↦ x ∈ m, Φ k x)
+    ([∗ map] k ↦ x ∈ m, Ψ1 k x) ([∗ map] k ↦ x ∈ m, Ψ2 k x).
 Proof.
   rewrite /FromSep=> ?. rewrite -big_sepM_sepM. by apply big_sepM_mono.
 Qed.
 Global Instance from_sep_big_sepS `{Countable A} (Φ Ψ1 Ψ2 : A → uPred M) X :
   (∀ x, FromSep (Φ x) (Ψ1 x) (Ψ2 x)) →
-  FromSep ([★ set] x ∈ X, Φ x) ([★ set] x ∈ X, Ψ1 x) ([★ set] x ∈ X, Ψ2 x).
+  FromSep ([∗ set] x ∈ X, Φ x) ([∗ set] x ∈ X, Ψ1 x) ([∗ set] x ∈ X, Ψ2 x).
 Proof.
   rewrite /FromSep=> ?. rewrite -big_sepS_sepS. by apply big_sepS_mono.
 Qed.
@@ -194,7 +194,7 @@ Global Instance into_op_Some {A : cmraT} (a : A) b1 b2 :
 Proof. by constructor. Qed.
 
 (* IntoAnd *)
-Global Instance into_and_sep p P Q : IntoAnd p (P ★ Q) P Q.
+Global Instance into_and_sep p P Q : IntoAnd p (P ∗ Q) P Q.
 Proof. by apply mk_into_and_sep. Qed.
 Global Instance into_and_ownM p (a b1 b2 : M) :
   IntoOp a b1 b2 →
@@ -217,8 +217,8 @@ Proof. rewrite /IntoAnd=>->. destruct p; by rewrite ?later_and ?later_sep. Qed.
 Global Instance into_and_big_sepM
     `{Countable K} {A} (Φ Ψ1 Ψ2 : K → A → uPred M) p m :
   (∀ k x, IntoAnd p (Φ k x) (Ψ1 k x) (Ψ2 k x)) →
-  IntoAnd p ([★ map] k ↦ x ∈ m, Φ k x)
-    ([★ map] k ↦ x ∈ m, Ψ1 k x) ([★ map] k ↦ x ∈ m, Ψ2 k x).
+  IntoAnd p ([∗ map] k ↦ x ∈ m, Φ k x)
+    ([∗ map] k ↦ x ∈ m, Ψ1 k x) ([∗ map] k ↦ x ∈ m, Ψ2 k x).
 Proof.
   rewrite /IntoAnd=> HΦ. destruct p.
   - apply and_intro; apply big_sepM_mono; auto.
@@ -228,7 +228,7 @@ Proof.
 Qed.
 Global Instance into_and_big_sepS `{Countable A} (Φ Ψ1 Ψ2 : A → uPred M) p X :
   (∀ x, IntoAnd p (Φ x) (Ψ1 x) (Ψ2 x)) →
-  IntoAnd p ([★ set] x ∈ X, Φ x) ([★ set] x ∈ X, Ψ1 x) ([★ set] x ∈ X, Ψ2 x).
+  IntoAnd p ([∗ set] x ∈ X, Φ x) ([∗ set] x ∈ X, Ψ1 x) ([∗ set] x ∈ X, Ψ2 x).
 Proof.
   rewrite /IntoAnd=> HΦ. destruct p.
   - apply and_intro; apply big_sepS_mono; auto.
@@ -243,18 +243,18 @@ Proof. by rewrite /Frame right_id. Qed.
 Global Instance frame_here_pure φ Q : FromPure Q φ → Frame (■ φ) Q True.
 Proof. rewrite /FromPure /Frame=> ->. by rewrite right_id. Qed.
 
-Class MakeSep (P Q PQ : uPred M) := make_sep : P ★ Q ⊣⊢ PQ.
+Class MakeSep (P Q PQ : uPred M) := make_sep : P ∗ Q ⊣⊢ PQ.
 Global Instance make_sep_true_l P : MakeSep True P P.
 Proof. by rewrite /MakeSep left_id. Qed.
 Global Instance make_sep_true_r P : MakeSep P True P.
 Proof. by rewrite /MakeSep right_id. Qed.
-Global Instance make_sep_default P Q : MakeSep P Q (P ★ Q) | 100.
+Global Instance make_sep_default P Q : MakeSep P Q (P ∗ Q) | 100.
 Proof. done. Qed.
 Global Instance frame_sep_l R P1 P2 Q Q' :
-  Frame R P1 Q → MakeSep Q P2 Q' → Frame R (P1 ★ P2) Q' | 9.
+  Frame R P1 Q → MakeSep Q P2 Q' → Frame R (P1 ∗ P2) Q' | 9.
 Proof. rewrite /Frame /MakeSep => <- <-. by rewrite assoc. Qed.
 Global Instance frame_sep_r R P1 P2 Q Q' :
-  Frame R P2 Q → MakeSep P1 Q Q' → Frame R (P1 ★ P2) Q' | 10.
+  Frame R P2 Q → MakeSep P1 Q Q' → Frame R (P1 ∗ P2) Q' | 10.
 Proof. rewrite /Frame /MakeSep => <- <-. by rewrite assoc (comm _ R) assoc. Qed.
 
 Class MakeAnd (P Q PQ : uPred M) := make_and : P ∧ Q ⊣⊢ PQ.
@@ -283,7 +283,7 @@ Global Instance frame_or R P1 P2 Q1 Q2 Q :
 Proof. rewrite /Frame /MakeOr => <- <- <-. by rewrite -sep_or_l. Qed.
 
 Global Instance frame_wand R P1 P2 Q2 :
-  Frame R P2 Q2 → Frame R (P1 -★ P2) (P1 -★ Q2).
+  Frame R P2 Q2 → Frame R (P1 -∗ P2) (P1 -∗ Q2).
 Proof.
   rewrite /Frame=> ?. apply wand_intro_l.
   by rewrite assoc (comm _ P1) -assoc wand_elim_r.
@@ -370,7 +370,7 @@ Proof. apply except_0_intro. Qed.
 
 (* ElimModal *)
 Global Instance elim_modal_wand P P' Q Q' R :
-  ElimModal P P' Q Q' → ElimModal P P' (R -★ Q) (R -★ Q').
+  ElimModal P P' Q Q' → ElimModal P P' (R -∗ Q) (R -∗ Q').
 Proof.
   rewrite /ElimModal=> H. apply wand_intro_r.
   by rewrite wand_curry -assoc (comm _ P') -wand_curry wand_elim_l.
@@ -389,13 +389,13 @@ Proof. by rewrite /ElimModal bupd_frame_r wand_elim_r bupd_trans. Qed.
 
 Global Instance elim_modal_except_0 P Q : IsExcept0 Q → ElimModal (◇ P) P Q Q.
 Proof.
-  intros. rewrite /ElimModal (except_0_intro (_ -★ _)).
+  intros. rewrite /ElimModal (except_0_intro (_ -∗ _)).
   by rewrite -except_0_sep wand_elim_r.
 Qed.
 Global Instance elim_modal_timeless_bupd P Q :
   TimelessP P → IsExcept0 Q → ElimModal (▷ P) P Q Q.
 Proof.
-  intros. rewrite /ElimModal (except_0_intro (_ -★ _)) (timelessP P).
+  intros. rewrite /ElimModal (except_0_intro (_ -∗ _)) (timelessP P).
   by rewrite -except_0_sep wand_elim_r.
 Qed.
 
