proofmode/notation.v
@@ -10,15 +10,15 @@ Notation "​" := Enil (format "​") : proof_scope.
 Notation "Γ ​ H : P" := (Esnoc Γ H P)
   (at level 1, P at level 200,
    left associativity, format "Γ ​ H  :  P '//'") : proof_scope.
-Notation "Γ '--------------------------------------' □ Δ '--------------------------------------' ★ Q" :=
+Notation "Γ '--------------------------------------' □ Δ '--------------------------------------' ∗ Q" :=
   (of_envs (Envs Γ Δ) ⊢ Q%I)
   (at level 1, Q at level 200, left associativity,
-  format "Γ '--------------------------------------' □ '//' Δ '--------------------------------------' ★ '//' Q '//'") :
+  format "Γ '--------------------------------------' □ '//' Δ '--------------------------------------' ∗ '//' Q '//'") :
   C_scope.
-Notation "Δ '--------------------------------------' ★ Q" :=
+Notation "Δ '--------------------------------------' ∗ Q" :=
   (of_envs (Envs Enil Δ) ⊢ Q%I)
   (at level 1, Q at level 200, left associativity,
-  format "Δ '--------------------------------------' ★ '//' Q '//'") : C_scope.
+  format "Δ '--------------------------------------' ∗ '//' Q '//'") : C_scope.
 Notation "Γ '--------------------------------------' □ Q" :=
   (of_envs (Envs Γ Enil) ⊢ Q%I)
   (at level 1, Q at level 200, left associativity,
